formalism changes

Protocols.lean
@@ -1,4 +1,4 @@
-abbrev Agent := String 
+abbrev Agent := String
 
 inductive Message (σ : Nat) where
 | empty : Message σ
@@ -16,139 +16,163 @@ notation " # " t " # " => Message.text t
 notation " pk( " i " ) " => Message.publicKey i
 notation " sk( " i " ) " => Message.secretKey i
 notation " ⦃| " m " |⦄ " k  => Message.encrypt m k
-notation " ag( " i " ) " => Message.agent i 
-notation " text( " t " ) " => Message.text t 
+notation " ag( " i " ) " => Message.agent i
+notation " text( " t " ) " => Message.text t
 notation m₁ " ‖ " m₂ => Message.concat m₁ m₂
 
-inductive Action (σ : Nat) where 
-| send : Agent → Agent → Message σ → Action σ 
-| recv : Agent → Message σ → Action σ 
-| comp : Action σ → Action σ → Action σ 
-| reun : Action σ → Action σ → Action σ 
-deriving Repr, BEq 
+inductive Action (σ : Nat) where
+| send : Agent → Agent → Message σ → Action σ
+| recv : Agent → Message σ → Action σ
+| comp : Action σ → Action σ → Action σ
+| reun : Action σ → Action σ → Action σ
+deriving Repr, BEq
 
-notation " send " i ", " j " ( " μ " ) " => Action.send i j μ 
-notation " recv " i " ( " μ " ) " => Action.recv i μ 
-notation α₁ " ; " α₂ => Action.comp α₁ α₂ 
-notation α₁ " ∪∪ " α₂ => Action.reun α₁ α₂ 
+notation " send " i ", " j " ( " μ " ) " => Action.send i j μ
+notation " recv " i " ( " μ " ) " => Action.recv i μ
+notation α₁ " ; " α₂ => Action.comp α₁ α₂
+notation α₁ " ∪∪ " α₂ => Action.reun α₁ α₂
 
-inductive State (σ : Nat) where 
-| explicit : Agent → Message σ → State σ 
-| add : State σ → State σ → State σ
-deriving Repr, BEq 
+inductive State (σ : Nat) where
+| explicit : Agent → Message σ → State σ
+| add : Agent → Message σ → State σ → State σ
+deriving Repr, BEq
 
-notation a " ▷ " μ => State.explicit a μ 
-notation γ₁ " ⊔ " γ₂ => State.add γ₁ γ₂ 
+notation a " ▷ " μ => State.explicit a μ
+notation a " ▷ " μ "⊔ " γ₁ => State.add a μ γ₁
 
-inductive Formula (σ : Nat) where 
+inductive Formula (σ : Nat) where
 | atom : Fin σ → Formula σ
-| true : Formula σ 
-| neg : Formula σ → Formula σ 
-| imp : Formula σ → Formula σ → Formula σ 
-| believe : Agent → Formula σ → Formula σ 
+| true : Formula σ
+| neg : Formula σ → Formula σ
+| imp : Formula σ → Formula σ → Formula σ
+| believe : Agent → Formula σ → Formula σ
 | explicit : Agent → Message σ → Formula σ
-| state2form : State σ → Formula σ 
-| state : Formula σ → Formula σ 
-| action : Action σ → Formula σ → Formula σ 
-deriving Repr, BEq 
+| state2form : State σ → Formula σ
+| state : Formula σ → Formula σ
+| action : Action σ → Formula σ → Formula σ
+deriving Repr, BEq
 
 notation " #ϕ " i => Formula.atom i
-notation " ⊤ " => Formula.true 
+notation " ⊤ " => Formula.true
 notation " ~ " φ => Formula.neg φ
 notation " ⊥ " => (~⊤)
 notation φ " ⟶ " ψ => Formula.imp φ ψ
 notation φ " ⋁ " ψ => ((~φ) ⟶ ψ)
 notation φ " ⋀ " ψ => ~((~φ) ⋁ (~ψ))
 notation " 𝔹 " i " , " φ => Formula.believe i φ
-notation " 𝕂 " i " , " φ => (𝔹 i, φ) ⋀ φ 
+notation " 𝕂 " i " , " φ => (𝔹 i, φ) ⋀ φ
 notation " 𝕏 " i " , " m => Formula.explicit i m
-notation " ι " γ => Formula.state2form γ 
-notation " ⟨ " γ " ⟩ " => Formula.state γ 
-notation " [ " α " ] " φ => Formula.action α φ 
+notation " ι " γ => Formula.state2form γ
+notation " ⟨ " γ " ⟩ " => Formula.state γ
+notation " [ " α " ] " φ => Formula.action α φ
 
-abbrev Context (σ : Nat) := List $ Formula σ 
+abbrev Context (σ : Nat) := List $ Formula σ
 
-inductive Proof {σ : Nat} : Context σ → Formula σ → Prop  
--- Hilbert basic 
-| ax { Γ } { p : Formula σ } (h : Γ.Mem p) : Proof Γ p 
+inductive Proof {σ : Nat} : Context σ → Formula σ → Prop
+-- Hilbert basic
+| ax { Γ } { p : Formula σ } (h : Γ.Mem p) : Proof Γ p
 | pl₁ { Γ } { p q : Formula σ } : Proof Γ (p ⟶ (q ⟶ p))
-| pl₂ { Γ } { p q r : Formula σ } : Proof Γ $ (p ⟶ (q ⟶ r)) ⟶ ((p ⟶ q) ⟶ (p ⟶ r)) 
+| pl₂ { Γ } { p q r : Formula σ } : Proof Γ $ (p ⟶ (q ⟶ r)) ⟶ ((p ⟶ q) ⟶ (p ⟶ r))
 | pl₃ { Γ } { p q : Formula σ } : Proof Γ $ ((~p) ⟶ ~q) ⟶ (q ⟶ p)
 -- K axiom for programs
 | Kα { Γ } { φ ψ : Formula σ } { α : Action σ } : Proof Γ $ ([α](φ ⟶ ψ)) ⟶ (([α]φ) ⟶ ([α]ψ))
--- Belief 
+-- Belief
 | K𝔹 { Γ } { φ ψ : Formula σ } { a : Agent } : Proof Γ $ (𝔹 a, (φ ⟶ ψ)) ⟶ ((𝔹 a, φ) ⟶ (𝔹 a, ψ))
 | D { Γ } { φ : Formula σ } {a : Agent} : Proof Γ $ (𝔹 a, φ) ⟶ ~(𝔹 a, (~φ))
-| _4 { Γ } { φ : Formula σ } {a : Agent} : Proof Γ $ (𝔹 a, φ) ⟶ (𝔹 a, (𝔹 a, φ)) 
-| _5 { Γ } { φ : Formula σ } {a : Agent} : Proof Γ $ (~(𝔹 a, φ)) ⟶ (𝔹 a, (~(𝔹 a, φ))) 
--- Deduction rules 
+| _4 { Γ } { φ : Formula σ } {a : Agent} : Proof Γ $ (𝔹 a, φ) ⟶ (𝔹 a, (𝔹 a, φ))
+| _5 { Γ } { φ : Formula σ } {a : Agent} : Proof Γ $ (~(𝔹 a, φ)) ⟶ (𝔹 a, (~(𝔹 a, φ)))
+-- Deduction rules
 | MP { Γ } { p q : Formula σ } (hpq : Proof Γ $ p ⟶ q) (hp : Proof Γ p) : Proof Γ q
-| NEC𝔹 { Γ } { φ : Formula σ } { a : Agent } (hφ : Proof Γ φ) : Proof Γ $ 𝔹 a, φ 
-| NECα { Γ } { φ : Formula σ } { α : Action σ } (hφ : Proof Γ φ) : Proof Γ $ [α]φ 
--- Actions 
+| NEC𝔹 { Γ } { φ : Formula σ } { a : Agent } (hφ : Proof Γ φ) : Proof Γ $ 𝔹 a, φ
+| NECα { Γ } { φ : Formula σ } { α : Action σ } (hφ : Proof Γ φ) : Proof Γ $ [α]φ
+-- Actions
 | Acomp_left { Γ } {α₁ α₂ : Action σ } { φ : Formula σ } : Proof Γ $ ([α₁ ; α₂]φ) ⟶ [α₁]([α₂]φ)
-| Acopm_right { Γ } {α₁ α₂ : Action σ } { φ : Formula σ } : Proof Γ $ [α₁]([α₂]φ) ⟶ ([α₁ ; α₂]φ)
--- States 
-| St₁_left { Γ } { γ₁ γ₂ : State σ } { a : Agent } { m : Message σ } : Proof Γ $ (ι (γ₁ ⊔ ((a ▷ m) ⊔ γ₂))) ⟶ ι ((a ▷ m) ⊔ (γ₁ ⊔ γ₂))
-| St₁_right { Γ } { γ₁ γ₂ : State σ } { a : Agent } { m : Message σ } : Proof Γ $ (ι ((a ▷ m) ⊔ (γ₁ ⊔ γ₂))) ⟶  ι (γ₁ ⊔ ((a ▷ m) ⊔ γ₂))
-| St₂_left { Γ } { γ : State σ } { a : Agent } { m : Message σ } : Proof Γ $ (ι ((a ▷ m) ⊔ ((a ▷ m) ⊔ γ))) ⟶  ι ((a ▷ m) ⊔ γ)
-| St₂_right { Γ } { γ : State σ } { a : Agent } { m : Message σ } : Proof Γ $ (ι ((a ▷ m) ⊔ γ)) ⟶ ι ((a ▷ m) ⊔ ((a ▷ m) ⊔ γ))
-| St₃ { Γ } { γ : State σ } { a : Agent } { m : Message σ } : Proof Γ $ (ι ((a ▷ m) ⊔ γ)) ⟶ 𝕏 a, m
+| Acomp_right { Γ } {α₁ α₂ : Action σ } { φ : Formula σ } : Proof Γ $ ([α₁]([α₂]φ)) ⟶ ([α₁ ; α₂]φ)
+-- States
+| St₁_left { Γ } { γ₂ : State σ } { a b : Agent } { m₁ m₂ : Message σ } : Proof Γ $ ⟨ι (a ▷ m₁ ⊔ b ▷ m₂ ⊔ γ₂)⟩ ⟶ ⟨ι (b ▷ m₂ ⊔ a ▷ m₁ ⊔ γ₂)⟩
+-- | St₁_right { Γ } { γ₁ γ₂ : State σ } { a : Agent } { m : Message σ } : Proof Γ $ (ι (a ▷ m ⊔ (γ₁ ⊔ γ₂))) ⟶  ι (γ₁ ⊔ ((a ▷ m) ⊔ γ₂))
+| St₂_left { Γ } { γ : State σ } { a : Agent } { m : Message σ } : Proof Γ $ (ι (a ▷ m ⊔ (a ▷ m ⊔ γ))) ⟶  ι (a ▷ m ⊔ γ)
+| St₂_right { Γ } { γ : State σ } { a : Agent } { m : Message σ } : Proof Γ $ (ι (a ▷ m ⊔ γ)) ⟶ ι (a ▷ m ⊔ (a ▷ m ⊔ γ))
+| St₃ { Γ } { γ : State σ } { a : Agent } { m : Message σ } : Proof Γ $ ⟨ ι (a ▷ m ⊔ γ) ⟩  ⟶ 𝕏 a, m
 -- theorems
-| St₁_left' { Γ } { γ₁ γ₂ : State σ } { a : Agent } { m : Message σ } : Proof Γ $ ⟨ι (γ₁ ⊔ ((a ▷ m) ⊔ γ₂))⟩ ⟶  ⟨ι ((a ▷ m) ⊔ (γ₁ ⊔ γ₂))⟩
-| St₁_right' { Γ } { γ₁ γ₂ : State σ } { a : Agent } { m : Message σ } : Proof Γ $ ⟨ι ((a ▷ m) ⊔ (γ₁ ⊔ γ₂))⟩ ⟶  ⟨ι (γ₁ ⊔ ((a ▷ m) ⊔ γ₂))⟩
-| St₂_left' { Γ } { γ : State σ } { a : Agent } { m : Message σ } : Proof Γ $ ⟨ι ((a ▷ m) ⊔ ((a ▷ m) ⊔ γ))⟩ ⟶  ⟨ι ((a ▷ m) ⊔ γ)⟩
-| St₂_right' { Γ } { γ : State σ } { a : Agent } { m : Message σ } : Proof Γ $ ⟨ι ((a ▷ m) ⊔ γ)⟩ ⟶ ⟨ι ((a ▷ m) ⊔ ((a ▷ m) ⊔ γ))⟩
-| St₃' { Γ } { γ : State σ } { a : Agent } { m : Message σ } : Proof Γ $ ⟨ι ((a ▷ m) ⊔ γ)⟩ ⟶ ⟨𝕏 a, m⟩
+--| St₁_left' { Γ } { γ₁ γ₂ : State σ } { a : Agent } { m : Message σ } : Proof Γ $ ⟨ι (γ₁ ⊔ ((a ▷ m) ⊔ γ₂))⟩ ⟶  ⟨ι ((a ▷ m) ⊔ (γ₁ ⊔ γ₂))⟩
+--| St₁_right' { Γ } { γ₁ γ₂ : State σ } { a : Agent } { m : Message σ } : Proof Γ $ ⟨ι ((a ▷ m) ⊔ (γ₁ ⊔ γ₂))⟩ ⟶  ⟨ι (γ₁ ⊔ ((a ▷ m) ⊔ γ₂))⟩
+| St₂_left' { Γ } { γ : State σ } { a : Agent } { m : Message σ } : Proof Γ $ ⟨ι (a ▷ m ⊔ (a ▷ m ⊔ γ))⟩ ⟶  ⟨ι (a ▷ m ⊔ γ)⟩
+| St₂_right' { Γ } { γ : State σ } { a : Agent } { m : Message σ } : Proof Γ $ ⟨ι (a ▷ m ⊔ γ)⟩ ⟶ ⟨ι (a ▷ m ⊔ (a ▷ m ⊔ γ))⟩
 
-notation Γ " ⊢ " φ => Proof Γ φ 
+notation Γ " ⊢ " φ => Proof Γ φ
 
 /-
   **PROTOCOLS**
 -/
 
-open Formula 
-open Proof 
+open Formula
+open Proof
 
-inductive ProtocolProof { σ : Nat } : Context σ → Formula σ → Prop 
--- an extension of standard proofs  
-| base { Γ } { φ } (proof : Proof Γ φ) : ProtocolProof Γ φ 
--- messages  
+inductive ProtocolProof { σ : Nat } : Context σ → Formula σ → Prop
+-- an extension of standard proofs
+| base { Γ } { φ } (proof : Proof Γ φ) : ProtocolProof Γ φ
+-- messages
 | X₁_left { Γ } { a : Agent } { m₁ m₂ : Message σ } : ProtocolProof Γ $ (𝕏 a, (m₁.concat m₂)) ⟶ ((𝕏 a, m₁) ⋀ (𝕏 a, m₂))
 | X₁_right { Γ } { a : Agent }{ m₁ m₂ : Message σ } : ProtocolProof Γ $ ((𝕏 a, m₁) ⋀ (𝕏 a, m₂)) ⟶ (𝕏 a, (m₁.concat m₂))
 | X₂_left { Γ } { a b : Agent } { k : Message σ } : ProtocolProof Γ $ (𝕏 a, (Message.symmetricKey a b k)) ⟶ (𝕏 b, (Message.symmetricKey b a k))
 | X₂_right { Γ } { a b : Agent } { k : Message σ } : ProtocolProof Γ $ (𝕏 b, (Message.symmetricKey b a k)) ⟶ (𝕏 a, (Message.symmetricKey a b k))
-| X₃ { Γ } { a b : Agent } { m : Message σ } : ProtocolProof Γ $ ((𝕏 a, ⦃|m|⦄ pk(b)) ⋀ (𝕏 a, sk(b))) ⟶ (𝕏 a, m)
+| X₃ { Γ } { a b : Agent } { m : Message σ } : ProtocolProof Γ $ ((𝕏 a, ⦃|m|⦄ pk(b)) ⋀ (⟨ 𝕏 a, sk(b) ⟩)) ⟶ (𝕏 a, m)
 | X₄ { Γ } { a b : Agent } { m : Message σ } : ProtocolProof Γ $ ((𝕏 a, ⦃|m|⦄ sk(b)) ⋀ (𝕏 a, pk(b))) ⟶ (𝕏 a, m)
-| X₅ { Γ } { a : Agent } { m₁ m₂ : Message σ } : ProtocolProof Γ $ ((𝕏 a, m₁) ⋀ (𝕏 a, m₂)) ⟶ 𝕏 a, ⦃|m₁|⦄m₂ 
+| X₅ { Γ } { a : Agent } { m₁ m₂ : Message σ } : ProtocolProof Γ $ ((𝕏 a, m₁) ⋀ (𝕏 a, m₂)) ⟶ 𝕏 a, ⦃|m₁|⦄m₂
 | X₆ { Γ } { a b : Agent } { m k : Message σ } : ProtocolProof Γ $ ((𝕏 a, ⦃|m|⦄ (Message.symmetricKey a b k)) ⋀ (𝕏 a, (Message.symmetricKey a b k))) ⟶ (𝕏 a, m)
 | X₇ { Γ } { a : Agent } : ProtocolProof Γ $ (𝕏 a, ag(a))
 -- protocol general hypotheses
-| H₁ { Γ } { a b e : Agent } {m : Message σ } { γ : State σ } : ProtocolProof Γ $ ⟨ ι ((a ▷ m) ⊔ γ) ⟩ ⟶ [send a,b(⦃| ag(a) ‖  m |⦄pk(b))]⟨ ι ((e ▷ m) ⊔ ((a ▷ m) ⊔ γ)) ⟩ 
-| H₂ { Γ } { a b e : Agent } {m : Message σ } { γ : State σ } : ProtocolProof Γ $ ⟨ ι ((e ▷ m) ⊔ γ) ⟩ ⟶ [recv a(⦃| ag(b) ‖ m |⦄pk(a))]⟨ ι ((a ▷ m) ⊔ ((e ▷ m) ⊔ γ)) ⟩  
+| H₁ { Γ } { a b : Agent } {m : Message σ } { γ : State σ } : ProtocolProof Γ $ ⟨ ι (a ▷ m ⊔ γ) ⟩ ⟶ [send a,b(⦃| ag(a) ‖ m |⦄pk(b))]⟨ ι (a ▷ m ⊔ γ) ⟩
+| H₂ { Γ } { a b : Agent } {m : Message σ } { γ : State σ } : ProtocolProof Γ $ ⟨ ι (a ▷ m ⊔ γ) ⟩ ⟶ [recv b(⦃| ag(a) ‖ m |⦄pk(b))]⟨ ι (b ▷ m ⊔ a ▷ m ⊔ γ) ⟩
 
-notation Γ " ⊢ₚ " φ => ProtocolProof Γ φ 
+notation Γ " ⊢ₚ " φ => ProtocolProof Γ φ
 
-inductive OSSProof { σ : Nat } : Context σ → Formula σ → Prop 
-| base { Γ } { φ } (proof : ProtocolProof Γ φ) : OSSProof Γ φ 
-| S₁ { Γ } {a b : Agent } { m : Message σ } { γ : State σ } : OSSProof Γ $ ⟨ ι ((a ▷ m) ⊔ γ) ⟩ ⟶ [send a,b(⦃| ag(a) ‖  m |⦄pk(b))]𝔹 a, ⟨ 𝕏 b, m ⟩ 
-| S₁' { Γ } {a b : Agent } { m : Message σ } { γ : State σ } { α : Action σ } : OSSProof Γ $ ⟨ ι ((a ▷ m) ⊔ γ) ⟩ ⟶ [(send a,b(⦃| ag(a) ‖  m |⦄pk(b))) ; α]𝔹 a, ⟨ 𝕏 b, m ⟩ 
-| S₂ { Γ } { a b : Agent } { m : Message σ } { γ : State σ } : OSSProof Γ $ ⟨ ι γ ⟩ ⟶ [recv b(⦃| ag(a) ‖  m |⦄pk(b))]𝔹 b, ⟨ 𝕏 a, m ⟩ 
-| S₂' { Γ } { a b : Agent } { m : Message σ } { α : Action σ } : OSSProof Γ $ [(recv b(⦃| ag(a) ‖  m |⦄pk(b))) ; α]𝔹 b, ⟨ 𝕏 a, m ⟩ 
--- added to simplify 
+inductive OSSProof { σ : Nat } : Context σ → Formula σ → Prop
+| base { Γ } { φ } (proof : ProtocolProof Γ φ) : OSSProof Γ φ
+| S₁ { Γ } {a b : Agent } { m : Message σ } { γ : State σ } : OSSProof Γ $ ⟨ ι (a ▷ m ⊔ γ) ⟩ ⟶ [send a,b(⦃| ag(a) ‖  m |⦄pk(b))]𝔹 a, 𝕏 b, m
+| S₂ { Γ } { a b : Agent } { m : Message σ } { γ : State σ } : OSSProof Γ $ ⟨ ι γ ⟩ ⟶ [recv b(⦃| ag(a) ‖  m |⦄pk(b))]𝔹 b, 𝕏 a, m
+
+-- added to simplify
 | MP { Γ } { p q : Formula σ } (hpq : OSSProof Γ $ p ⟶ q) (hp : OSSProof Γ p) : OSSProof Γ q
-| NECα { Γ } { φ : Formula σ } { α : Action σ } (hφ : OSSProof Γ φ) : OSSProof Γ $ [α]φ 
+| NECα { Γ } { φ : Formula σ } { α : Action σ } (hφ : OSSProof Γ φ) : OSSProof Γ $ [α]φ
 
-notation Γ " ⊢ₒₛₛ " φ => OSSProof Γ φ 
+notation Γ " ⊢ₒₛₛ " φ => OSSProof Γ φ
 
+inductive OSSEProof { σ : Nat } : Context σ → Formula σ → Prop
+| base { Γ } { φ } (proof : OSSProof Γ φ) : OSSEProof Γ φ
+-- axioms which define the adversary (de intrebat)
+| H₁ₑ { Γ } { a b e : Agent } {m : Message σ } { γ : State σ } : OSSEProof Γ $ ⟨ ι (a ▷ m ⊔ γ) ⟩ ⟶ [send a,b(⦃| ag(a) ‖ m |⦄pk(b))]⟨ ι (e ▷ m ⊔ (a ▷ m ⊔ γ)) ⟩ -- nu am folosit-o
+| H₂ₑ { Γ } { a b e : Agent } {m : Message σ } { γ : State σ } { α : Action σ } : OSSEProof Γ $ ⟨ ι (e ▷ m ⊔ γ) ⟩ ⟶ [α ; recv b(⦃| ag(a) ‖ m |⦄pk(b))]⟨ ι (b ▷ m ⊔ (e ▷ m ⊔ γ)) ⟩
+| adv₁ { Γ } {a b e : Agent } { m : Message σ } { γ : State σ } { α : Action σ } : OSSEProof Γ $ ⟨ ι (e ▷ m ⊔ γ) ⟩ ⟶ [send e,b(⦃| ag(a) ‖  m |⦄pk(b)) ; α]𝕏 e, m
+| adv₂ { Γ } {a b e : Agent } { m : Message σ } { γ : State σ } { α : Action σ } : OSSEProof Γ $ ⟨ ι (e ▷ m ⊔ γ) ⟩ ⟶ [send e,b(⦃| ag(a) ‖  m |⦄pk(b)) ; α]𝔹 e, 𝕏 b, m
+-- de intrebat
+| H₁' { Γ } { a b e : Agent } {m : Message σ } { γ : State σ } : OSSEProof Γ $ ⟨ ι (e ▷ m ⊔ γ) ⟩ ⟶ [send e,b(⦃| ag(a) ‖ m |⦄pk(b))]⟨ ι (e ▷ m ⊔ γ) ⟩
 
-def γᵢₙᵢₜ {σ : Nat} {i r : Agent} : State σ := (i ▷ pk(i)) ⊔ (i ▷ sk(i)) ⊔ (i ▷ pk(i)) ⊔ (r ▷ sk(r))
+-- added to simplify
+| MP { Γ } { p q : Formula σ } (hpq : OSSEProof Γ $ p ⟶ q) (hp : OSSEProof Γ p) : OSSEProof Γ q
+
+notation Γ " ⊢ₒₛₛₑ " φ => OSSEProof Γ φ
+
+def γᵢₙᵢₜ {σ : Nat} {i r : Agent} : State σ := r ▷ sk(r) ⊔ r ▷ pk(i) ⊔ r ▷ pk(r) ⊔ i ▷ pk(i) ⊔ i ▷ sk(i) ⊔ i ▷ pk(r)
+def γᵢₙᵢₜₑ {σ : Nat} {i r e : Agent} : State σ := r ▷ sk(r) ⊔ r ▷ pk(i) ⊔ r ▷ pk(r) ⊔ r ▷ pk(e) ⊔
+                                                 i ▷ pk(i) ⊔ i ▷ sk(i) ⊔ i ▷ pk(r) ⊔ i ▷ pk(e) ⊔
+                                                 e ▷ sk(e) ⊔ e ▷ pk(e) ⊔ e ▷ pk(i) ⊔ e ▷ pk(r)
 
 @[simp]
-theorem pl_transitivity {σ : Nat} {p q r : Formula σ} { Γ : Context σ } : 
-  (Γ ⊢ₒₛₛ (p ⟶ q)) → 
-  (Γ ⊢ₒₛₛ (q ⟶ r)) → 
-  (Γ ⊢ₒₛₛ (p ⟶ r)) := by 
+theorem pl_transitivity {σ : Nat} {p q r : Formula σ} { Γ : Context σ } :
+  (Γ ⊢ (p ⟶ q)) → (Γ ⊢ (q ⟶ r)) → (Γ ⊢ (p ⟶ r)) := by
+  intros hpq hqr
+  have H₁ : Γ ⊢ (p ⟶ q ⟶ r) := Proof.MP Proof.pl₁ hqr
+  have H₂ : Γ ⊢ ((p ⟶ q ⟶ r) ⟶ (p ⟶ q) ⟶ (p ⟶ r)) := Proof.pl₂
+  have H₃ : Γ ⊢ ((p ⟶ q) ⟶ (p ⟶ r)) := Proof.MP H₂ H₁
+  exact Proof.MP H₃ hpq
+
+@[simp]
+theorem pl_transitivity_oss {σ : Nat} {p q r : Formula σ} { Γ : Context σ } :
+  (Γ ⊢ₒₛₛ (p ⟶ q)) →
+  (Γ ⊢ₒₛₛ (q ⟶ r)) →
+  (Γ ⊢ₒₛₛ (p ⟶ r)) := by
   intros hpq hqr
   have h₁ : Γ ⊢ₒₛₛ (p ⟶ q ⟶ r) :=
     OSSProof.MP
@@ -161,71 +185,260 @@ theorem pl_transitivity {σ : Nat} {p q r : Formula σ} { Γ : Context σ } :
   exact OSSProof.MP h₃ hpq
 
 @[simp]
-theorem dl_th_1 {σ : Nat} { p q r : Formula σ } { α : Action σ } { Γ : Context σ } : 
-  (Γ ⊢ₒₛₛ (p ⟶ ([α]q))) → 
-  (Γ ⊢ₒₛₛ (p ⟶ ([α]r))) → 
-  (Γ ⊢ₒₛₛ (p ⟶ ([α](q ⋀ r)))) := by 
-  admit 
-
+theorem pl_transitivity_osse {σ : Nat} {p q r : Formula σ} { Γ : Context σ } :
+  (Γ ⊢ₒₛₛₑ (p ⟶ q)) →
+  (Γ ⊢ₒₛₛₑ (q ⟶ r)) →
+  (Γ ⊢ₒₛₛₑ (p ⟶ r)) := by
+  intros hpq hqr
+  have h₁ : Γ ⊢ₒₛₛₑ (p ⟶ q ⟶ r) :=
+    OSSEProof.MP
+      (OSSEProof.base $ OSSProof.base (ProtocolProof.base Proof.pl₁))
+      hqr
+  have h₂ : Γ ⊢ₒₛₛₑ ((p ⟶ q ⟶ r) ⟶ (p ⟶ q) ⟶ (p ⟶ r)) :=
+    OSSEProof.base $ OSSProof.base (ProtocolProof.base Proof.pl₂)
+  have h₃ : Γ ⊢ₒₛₛₑ ((p ⟶ q) ⟶ (p ⟶ r)) :=
+    OSSEProof.MP h₂ h₁
+  exact OSSEProof.MP h₃ hpq
 
 @[simp]
-theorem dl_th_2 {σ : Nat} { p q r : Formula σ } { α β : Action σ } { Γ : Context σ } : 
-  (Γ ⊢ₒₛₛ (p ⟶ ([α][β](q ⋀ r)))) → 
-  (Γ ⊢ₒₛₛ (p ⟶ ([α][β]r))) := by 
-  intros h
+theorem pl2_aux {σ : Nat} {p q r : Formula σ} { Γ : Context σ } :
+  (Γ ⊢ₒₛₛ (p ⟶ q)) →
+  (Γ ⊢ₒₛₛ (p ⟶ q ⟶ r)) →
+  (Γ ⊢ₒₛₛ (p ⟶ r)) := by
+  intros hpq hpqr
+  exact OSSProof.MP (OSSProof.MP (OSSProof.base (ProtocolProof.base Proof.pl₂)) hpqr) hpq
 
+@[simp]
+theorem pl2_aux_e {σ : Nat} {p q r : Formula σ} { Γ : Context σ } :
+  (Γ ⊢ₒₛₛₑ (p ⟶ q)) →
+  (Γ ⊢ₒₛₛₑ (p ⟶ q ⟶ r)) →
+  (Γ ⊢ₒₛₛₑ (p ⟶ r)) := by
+  intros hpq hpqr
+  exact OSSEProof.MP (OSSEProof.MP (OSSEProof.base $ OSSProof.base (ProtocolProof.base Proof.pl₂)) hpqr) hpq
+
+@[simp]
+theorem dl_th_1 {σ : Nat} { p q r : Formula σ } { α : Action σ } { Γ : Context σ } :
+  (Γ ⊢ₒₛₛ (p ⟶ ([α]q))) →
+  (Γ ⊢ₒₛₛ (p ⟶ ([α]r))) →
+  (Γ ⊢ₒₛₛ (p ⟶ ([α](q ⋀ r)))) := by
+  intros hq hr
+  have prop_formula : Γ ⊢ (q ⟶ r ⟶ q ⋀ r) := by
+    admit
+  have nec_formula : Γ ⊢ₒₛₛ ([α](q ⟶ (r ⟶ q ⋀ r))) ⟶ ([α]q) ⟶ ([α](r ⟶ q ⋀ r)) := OSSProof.base (ProtocolProof.base Proof.Kα)
+  have h₀ : Γ ⊢ₒₛₛ ([α](q ⟶ (r ⟶ q ⋀ r))) := OSSProof.base (ProtocolProof.base (Proof.NECα prop_formula))
+  have h₁ : Γ ⊢ₒₛₛ ([α]q) ⟶ ([α](r ⟶ q ⋀ r)) := OSSProof.MP nec_formula h₀
+  have h₂ : Γ ⊢ₒₛₛ (p ⟶ ([α](r ⟶ q ⋀ r))) := pl_transitivity_oss hq h₁
+  have nec_formula : Γ ⊢ₒₛₛ ([α](r ⟶ q ⋀ r)) ⟶ ([α](r)) ⟶ ([α](q ⋀ r)) := OSSProof.base (ProtocolProof.base Proof.Kα)
+  have h₃ := pl_transitivity_oss h₂ nec_formula
+  exact pl2_aux hr h₃
+
+@[simp]
+theorem dl_th_1_e {σ : Nat} { p q r : Formula σ } { α : Action σ } { Γ : Context σ } :
+  (Γ ⊢ₒₛₛₑ (p ⟶ ([α]q))) →
+  (Γ ⊢ₒₛₛₑ (p ⟶ ([α]r))) →
+  (Γ ⊢ₒₛₛₑ (p ⟶ ([α](q ⋀ r)))) := by
+  intros hq hr
+  have prop_formula : Γ ⊢ (q ⟶ r ⟶ q ⋀ r) := by
+    admit
+  have nec_formula : Γ ⊢ₒₛₛₑ ([α](q ⟶ (r ⟶ q ⋀ r))) ⟶ ([α]q) ⟶ ([α](r ⟶ q ⋀ r)) := OSSEProof.base $ OSSProof.base (ProtocolProof.base Proof.Kα)
+  have h₀ : Γ ⊢ₒₛₛₑ ([α](q ⟶ (r ⟶ q ⋀ r))) := OSSEProof.base $ OSSProof.base (ProtocolProof.base (Proof.NECα prop_formula))
+  have h₁ : Γ ⊢ₒₛₛₑ ([α]q) ⟶ ([α](r ⟶ q ⋀ r)) := OSSEProof.MP nec_formula h₀
+  have h₂ : Γ ⊢ₒₛₛₑ (p ⟶ ([α](r ⟶ q ⋀ r))) := pl_transitivity_osse hq h₁
+  have nec_formula : Γ ⊢ₒₛₛₑ ([α](r ⟶ q ⋀ r)) ⟶ ([α](r)) ⟶ ([α](q ⋀ r)) := OSSEProof.base $ OSSProof.base (ProtocolProof.base Proof.Kα)
+  have h₃ := pl_transitivity_osse h₂ nec_formula
+  exact pl2_aux_e hr h₃
+
+@[simp]
+theorem dl_th_3 {σ : Nat} { p q : Formula σ } { α β : Action σ } { Γ : Context σ } :
+  (Γ ⊢ₒₛₛ (p ⟶ [α]([β]q))) →
+  (Γ ⊢ₒₛₛ (p ⟶ ([α ; β]q))) := by
+  intro Hαβ
+  exact pl_transitivity_oss Hαβ (OSSProof.base $ ProtocolProof.base $ Proof.Acomp_right)
+
+@[simp]
+theorem dl_th_4 {σ : Nat} { p q : Formula σ } { α β : Action σ } { Γ : Context σ } :
+  (Γ ⊢ₒₛₛ (p ⟶ ([α ; β]q))) →
+  (Γ ⊢ₒₛₛ (p ⟶ [α]([β]q))) := by
+  intro Hαβ
+  exact pl_transitivity_oss Hαβ (OSSProof.base $ ProtocolProof.base $ Proof.Acomp_left)
+
+@[simp]
+theorem reductio_ad_absurdum {σ : Nat} { p q : Formula σ } { Γ : Context σ } : (Γ ⊢ ((~q) ⟶ (~(p ⟶ p)))) → (Γ ⊢ q) := by
+  intro H
+  exact Proof.MP (Proof.MP Proof.pl₃ H) (Proof.MP (Proof.MP Proof.pl₂ Proof.pl₁) (@Proof.pl₁ _ _ p p))
+
+@[simp]
+theorem premises_comm {σ : Nat} { p q r : Formula σ } { Γ : Context σ } : (Γ ⊢ (p ⟶ (q ⟶ r))) → (Γ ⊢ (q ⟶ (p ⟶ r))) := by
+  intro H
+  exact Proof.MP (Proof.MP Proof.pl₂ (Proof.MP Proof.pl₁ (Proof.MP Proof.pl₂ H))) Proof.pl₁
+
+@[simp]
+theorem contradiction {σ : Nat} { p q : Formula σ } { Γ : Context σ } : Γ ⊢ (q ⟶ ((~q) ⟶ p)) :=
+  premises_comm (pl_transitivity Proof.pl₁ Proof.pl₃)
+
+@[simp]
+theorem dne {σ : Nat} { p : Formula σ } { Γ : Context σ } : Γ ⊢ ((~(~p)) ⟶ p) := by admit
+
+@[simp]
+theorem rec_ax3 {σ : Nat} { p q : Formula σ } { Γ : Context σ }: Γ ⊢ (p ⟶ q) ⟶ ((~q) ⟶ (~p)) := by admit
+
+@[simp]
+theorem dl_th_2 {σ : Nat} { p q r : Formula σ } { α β : Action σ } { Γ : Context σ } :
+  (Γ ⊢ₒₛₛ (p ⟶ ([α][β](q ⋀ r)))) →
+  (Γ ⊢ₒₛₛ (p ⟶ ([α][β]r))) := by
+  intros h
   have prop_formula : Γ ⊢ ((q ⋀ r) ⟶ r) := by
-    admit 
-  have nec_formula : Γ ⊢ [α][β]((q ⋀ r) ⟶ r) := Proof.NECα (Proof.NECα prop_formula)
-  have nec_formula' : Γ ⊢ₒₛₛ [α][β]((q ⋀ r) ⟶ r) :=
-    OSSProof.base (ProtocolProof.base nec_formula)
-  admit 
+    have H₁ : Γ ⊢ ((~r) ⟶ ((~q) ⋁ (~r))) := Proof.pl₁
+    let Hmp := Proof.MP rec_ax3 H₁
+    exact (pl_transitivity Hmp (@dne _ r _))
+  have nec_formula : Γ ⊢ₒₛₛ [α ; β]((q ⋀ r) ⟶ r) := OSSProof.base $ ProtocolProof.base (Proof.NECα prop_formula)
+  let nec_formula_K := OSSProof.base $ ProtocolProof.base $ @Proof.Kα _ Γ (q ⋀ r) r (α ; β)
+  let HMP := OSSProof.MP nec_formula_K nec_formula
+  let Htrans := dl_th_3 h
+  exact (pl_transitivity_oss Htrans (dl_th_4 HMP))
+
 
 @[simp]
-theorem dl_th_3 {σ : Nat} { p q : Formula σ } { α β : Action σ } { Γ : Context σ } : 
-  (Γ ⊢ₒₛₛ (p ⟶ ([α]([β]q)))) → 
-  (Γ ⊢ₒₛₛ (p ⟶ ([α ; β]q))) := by 
-  admit 
+theorem pl_aux {σ : Nat} {p q r : Formula σ} { Γ : Context σ } :
+  (Γ ⊢ₒₛₛ (p ⟶ q)) →
+  (Γ ⊢ₒₛₛ (r ⋀ p) ⟶ (r ⋀ q)) := by
+  intros hpq
+  admit
+
+theorem oss { σ : Nat } { Γ : Context σ } { i r : Agent } { nᵢ : Message σ } :
+  Γ ⊢ₒₛₛ ⟨ ι (i ▷ nᵢ ⊔ (@γᵢₙᵢₜ σ i r)) ⟩
+    ⟶ [(send i, r(⦃| ag(i) ‖ nᵢ |⦄pk(r))) ; (recv r(⦃| ag(i) ‖ nᵢ |⦄pk(r)))](𝕂 r, 𝕏 i, nᵢ ) :=  by
+  have H₁ : Γ ⊢ₒₛₛ ⟨ ι (i ▷ nᵢ ⊔ (@γᵢₙᵢₜ σ i r)) ⟩ ⟶ [send i,r(⦃| ag(i) ‖ nᵢ |⦄pk(r))](𝔹 i, 𝕏 r, nᵢ)
+    := OSSProof.S₁
+  have H₂ : Γ ⊢ₒₛₛ ⟨ ι (i ▷ nᵢ ⊔ (@γᵢₙᵢₜ σ i r)) ⟩ ⟶ [send i,r(⦃| ag(i) ‖ nᵢ |⦄pk(r))]⟨ ι (i ▷ nᵢ ⊔ (@γᵢₙᵢₜ σ i r))⟩
+    := OSSProof.base $ ProtocolProof.H₁
+  have H₃ : Γ ⊢ₒₛₛ ⟨ ι (i ▷ nᵢ ⊔ (@γᵢₙᵢₜ σ i r)) ⟩ ⟶ [send i,r(⦃| ag(i) ‖ nᵢ |⦄pk(r))](𝔹 i,  𝕏 r, nᵢ ) ⋀ ⟨ ι (i ▷ nᵢ ⊔ (@γᵢₙᵢₜ σ i r))⟩
+    := dl_th_1 H₁ H₂
+  have H₄ : Γ ⊢ₒₛₛ ⟨ ι (i ▷ nᵢ ⊔ (@γᵢₙᵢₜ σ i r)) ⟩ ⟶ [recv r(⦃| ag(i) ‖ nᵢ |⦄pk(r))](𝔹 r, 𝕏 i, nᵢ )
+    := OSSProof.S₂
+  have H₅ : Γ ⊢ₒₛₛ ⟨ ι (i ▷ nᵢ ⊔ (@γᵢₙᵢₜ σ i r)) ⟩ ⟶ [recv r(⦃| ag(i) ‖ nᵢ |⦄pk(r))]⟨ ι (r ▷ nᵢ ⊔ i ▷ nᵢ ⊔ (@γᵢₙᵢₜ σ i r))⟩
+    := OSSProof.base $ ProtocolProof.H₂
+  have H₆ : Γ ⊢ₒₛₛ ⟨ ι (i ▷ nᵢ ⊔ (@γᵢₙᵢₜ σ i r)) ⟩ ⟶ [recv r(⦃| ag(i) ‖ nᵢ |⦄pk(r))](𝔹 r, 𝕏 i, nᵢ ) ⋀ ⟨ ι (r ▷ nᵢ ⊔ i ▷ nᵢ ⊔ (@γᵢₙᵢₜ σ i r))⟩
+    := dl_th_1 H₄ H₅
+  have H₇ : Γ ⊢ₒₛₛ [send i,r(⦃| ag(i) ‖ nᵢ |⦄pk(r))]⟨ ι (i ▷ nᵢ ⊔ (@γᵢₙᵢₜ σ i r)) ⟩ ⟶ [recv r(⦃| ag(i) ‖ nᵢ |⦄pk(r))](𝔹 r, 𝕏 i, nᵢ ) ⋀ ⟨ ι (r ▷ nᵢ ⊔ i ▷ nᵢ ⊔ (@γᵢₙᵢₜ σ i r))⟩
+    := OSSProof.NECα H₆
+  have H₈ : Γ ⊢ₒₛₛ ([send i,r(⦃| ag(i) ‖ nᵢ |⦄pk(r))]⟨ ι (i ▷ nᵢ ⊔ (@γᵢₙᵢₜ σ i r)) ⟩ ⟶ [recv r(⦃| ag(i) ‖ nᵢ |⦄pk(r))](𝔹 r, 𝕏 i, nᵢ) ⋀ ⟨ ι (r ▷ nᵢ ⊔ i ▷ nᵢ ⊔ (@γᵢₙᵢₜ σ i r))⟩) ⟶
+            ([send i,r(⦃| ag(i) ‖ nᵢ |⦄pk(r))]⟨ ι (i ▷ nᵢ ⊔ (@γᵢₙᵢₜ σ i r)) ⟩) ⟶ ([send i,r(⦃| ag(i) ‖ nᵢ |⦄pk(r))][recv r(⦃| ag(i) ‖ nᵢ |⦄pk(r))](𝔹 r, 𝕏 i, nᵢ) ⋀ ⟨ ι (r ▷ nᵢ ⊔ i ▷ nᵢ ⊔ (@γᵢₙᵢₜ σ i r))⟩)
+    := OSSProof.base $ ProtocolProof.base $ Proof.Kα
+  have H₉ : Γ ⊢ₒₛₛ ⟨ι (r ▷ nᵢ ⊔ i ▷ nᵢ ⊔ (@γᵢₙᵢₜ σ i r))⟩ ⟶ ⟨ι (i ▷ nᵢ ⊔ r ▷ nᵢ ⊔ (@γᵢₙᵢₜ σ i r))⟩
+    := OSSProof.base $ ProtocolProof.base $ Proof.St₁_left
+  have H₁₀ : Γ ⊢ₒₛₛ ⟨ι (i ▷ nᵢ ⊔ r ▷ nᵢ ⊔ (@γᵢₙᵢₜ σ i r))⟩ ⟶ 𝕏 i, nᵢ
+    := OSSProof.base $ ProtocolProof.base $ Proof.St₃
+  have H₁₁ : Γ ⊢ₒₛₛ [send i,r(⦃| ag(i) ‖ nᵢ |⦄pk(r)) ; recv r(⦃| ag(i) ‖ nᵢ |⦄pk(r))]((𝔹 r, 𝕏 i, nᵢ) ⋀ ⟨ ι (r ▷ nᵢ ⊔ i ▷ nᵢ ⊔ (@γᵢₙᵢₜ σ i r))⟩) ⟶ ((𝔹 r, 𝕏 i, nᵢ) ⋀ 𝕏 i, nᵢ)
+    := OSSProof.NECα (pl_aux (pl_transitivity_oss H₉ H₁₀))
+  let H₁₂ := OSSProof.base $ ProtocolProof.base $ @Proof.Kα _ Γ ((𝔹 r, 𝕏 i, nᵢ) ⋀ ⟨ ι (r ▷ nᵢ ⊔ i ▷ nᵢ ⊔ (@γᵢₙᵢₜ σ i r))⟩) ((𝔹 r, 𝕏 i, nᵢ) ⋀ 𝕏 i, nᵢ) (send i,r(⦃| ag(i) ‖ nᵢ |⦄pk(r)) ; recv r(⦃| ag(i) ‖ nᵢ |⦄pk(r)))
+  exact pl_transitivity_oss (dl_th_3 $ pl_transitivity_oss H₂ (OSSProof.MP H₈ H₇)) (OSSProof.MP H₁₂ H₁₁)
+
+theorem oss_mitm { σ : Nat } { Γ : Context σ } { i r e : Agent } { nₑ : Message σ } :
+  Γ ⊢ₒₛₛₑ ⟨ ι (e ▷ nₑ ⊔ (@γᵢₙᵢₜₑ σ i r e)) ⟩
+    ⟶ [(send e, r(⦃| ag(i) ‖ nₑ |⦄pk(r))) ; (recv r(⦃| ag(i) ‖ nₑ |⦄pk(r)))](((𝕂 e, 𝕏 r, nₑ) ⋀ (𝕏 e, nₑ)) ⋀ (𝔹 r, 𝕏 i, nₑ)) := by
+  have H₁ : Γ ⊢ₒₛₛₑ ⟨ ι (e ▷ nₑ ⊔ (@γᵢₙᵢₜₑ σ i r e)) ⟩ ⟶ [send e,r(⦃| ag(i) ‖ nₑ |⦄pk(r))]⟨ ι (e ▷ nₑ ⊔ (@γᵢₙᵢₜₑ σ i r e)) ⟩
+    := OSSEProof.H₁'
+  have H₂ : Γ ⊢ₒₛₛ ⟨ ι (e ▷ nₑ ⊔ (@γᵢₙᵢₜₑ σ i r e)) ⟩ ⟶ [(recv r(⦃| ag(i) ‖ nₑ |⦄pk(r)))](𝔹 r, 𝕏 i, nₑ)
+    := OSSProof.S₂
+  have H₃ : Γ ⊢ₒₛₛ [(send e, r(⦃| ag(i) ‖ nₑ |⦄pk(r)))]⟨ ι (e ▷ nₑ ⊔ (@γᵢₙᵢₜₑ σ i r e)) ⟩ ⟶ [(recv r(⦃| ag(i) ‖ nₑ |⦄pk(r)))](𝔹 r, 𝕏 i, nₑ)
+    := OSSProof.NECα H₂
+  have H₄ : Γ ⊢ₒₛₛ ([(send e, r(⦃| ag(i) ‖ nₑ |⦄pk(r)))]⟨ ι (e ▷ nₑ ⊔ (@γᵢₙᵢₜₑ σ i r e)) ⟩ ⟶ [(recv r(⦃| ag(i) ‖ nₑ |⦄pk(r)))](𝔹 r, 𝕏 i, nₑ)) ⟶
+                  ([(send e, r(⦃| ag(i) ‖ nₑ |⦄pk(r)))]⟨ ι (e ▷ nₑ ⊔ (@γᵢₙᵢₜₑ σ i r e)) ⟩) ⟶ ([(send e, r(⦃| ag(i) ‖ nₑ |⦄pk(r)))][(recv r(⦃| ag(i) ‖ nₑ |⦄pk(r)))](𝔹 r, 𝕏 i, nₑ))
+    := OSSProof.base $ ProtocolProof.base $ Proof.Kα
+  have H₅ : Γ ⊢ₒₛₛₑ ⟨ ι (e ▷ nₑ ⊔ (@γᵢₙᵢₜₑ σ i r e)) ⟩ ⟶ [(send e, r(⦃| ag(i) ‖ nₑ |⦄pk(r))) ; (recv r(⦃| ag(i) ‖ nₑ |⦄pk(r)))]𝕏 e, nₑ
+    := OSSEProof.adv₁
+  have H₆ : Γ ⊢ₒₛₛₑ ⟨ ι (e ▷ nₑ ⊔ (@γᵢₙᵢₜₑ σ i r e)) ⟩ ⟶ [(send e, r(⦃| ag(i) ‖ nₑ |⦄pk(r))) ; (recv r(⦃| ag(i) ‖ nₑ |⦄pk(r)))]𝔹 e, 𝕏 r, nₑ
+    := OSSEProof.adv₂
+  have H₇ : Γ ⊢ₒₛₛₑ ⟨ ι (e ▷ nₑ ⊔ (@γᵢₙᵢₜₑ σ i r e)) ⟩ ⟶ [(send e, r(⦃| ag(i) ‖ nₑ |⦄pk(r))) ; (recv r(⦃| ag(i) ‖ nₑ |⦄pk(r)))]⟨ ι (r ▷ nₑ ⊔ (e ▷ nₑ ⊔ (@γᵢₙᵢₜₑ σ i r e))) ⟩
+    := OSSEProof.H₂ₑ
+  have H₈ : Γ ⊢ₒₛₛ ⟨ ι (r ▷ nₑ ⊔ (e ▷ nₑ ⊔ (@γᵢₙᵢₜₑ σ i r e))) ⟩ ⟶ 𝕏 r, nₑ
+    := OSSProof.base $ ProtocolProof.base $ Proof.St₃
+  have H₉ : Γ ⊢ₒₛₛ [(send e, r(⦃| ag(i) ‖ nₑ |⦄pk(r))) ; (recv r(⦃| ag(i) ‖ nₑ |⦄pk(r)))]⟨ ι (r ▷ nₑ ⊔ (e ▷ nₑ ⊔ (@γᵢₙᵢₜₑ σ i r e))) ⟩ ⟶ 𝕏 r, nₑ
+    := OSSProof.NECα H₈
+  have H₁₀ : Γ ⊢ₒₛₛ ([(send e, r(⦃| ag(i) ‖ nₑ |⦄pk(r))) ; (recv r(⦃| ag(i) ‖ nₑ |⦄pk(r)))]⟨ ι (r ▷ nₑ ⊔ (e ▷ nₑ ⊔ (@γᵢₙᵢₜₑ σ i r e))) ⟩ ⟶ 𝕏 r, nₑ) ⟶
+                   ([(send e, r(⦃| ag(i) ‖ nₑ |⦄pk(r))) ; (recv r(⦃| ag(i) ‖ nₑ |⦄pk(r)))]⟨ ι (r ▷ nₑ ⊔ (e ▷ nₑ ⊔ (@γᵢₙᵢₜₑ σ i r e))) ⟩) ⟶
+                   ([(send e, r(⦃| ag(i) ‖ nₑ |⦄pk(r))) ; (recv r(⦃| ag(i) ‖ nₑ |⦄pk(r)))] 𝕏 r, nₑ)
+    := OSSProof.base $ ProtocolProof.base $ Proof.Kα
+  exact dl_th_1_e (dl_th_1_e (dl_th_1_e H₆ (pl_transitivity_osse H₇ (OSSEProof.base $ OSSProof.MP H₁₀ H₉))) H₅) (pl_transitivity_osse H₁ (OSSEProof.base $ dl_th_3 $ OSSProof.MP H₄ H₃))
+
+inductive NSProof { σ : Nat } : Context σ → Formula σ → Prop
+| base { Γ } { φ } (proof : ProtocolProof Γ φ) : NSProof Γ φ
+
+| S₁ { Γ } {a b : Agent } { m : Message σ } { γ : State σ } {α : Action σ} : NSProof Γ $ ⟨ ι (a ▷ m ⊔ γ) ⟩ ⟶ [send a,b(⦃| ag(a) ‖  m |⦄pk(b)); α]𝔹 a, (𝕏 b, m)
+| S₂ { Γ } { a b : Agent } { m₁ m₂ : Message σ } { γ : State σ } {α : Action σ} : NSProof Γ $ ⟨ ι (b ▷ m₂ ⊔ γ) ⟩ ⋀ 𝔹 a, (𝕏 b, m₁) ⟶ [send b,a(⦃| m₁ ‖  m₂ |⦄pk(a))]𝔹 b, (𝕏 a, m₂)
+| S₃ { Γ } { a b : Agent } { m₂ : Message σ } {α : Action σ} : NSProof Γ $ 𝔹 b, ⟨ 𝕏 a, m₂ ⟩ ⟶ [send a,b(⦃| m₂ |⦄pk(b)); α](𝕏 a, m₂)
+
+| R₁ { Γ } {a b : Agent } { m : Message σ } { γ : State σ } {α : Action σ} : NSProof Γ $ ⟨ ι γ ⟩ ⟶ [α ; recv b(⦃| ag(a) ‖  m |⦄pk(b))]𝔹 b, (𝕏 a, m)
+| R₁' { Γ } {a b : Agent } { m : Message σ } { γ : State σ } : NSProof Γ $ ⟨ ι γ ⟩ ⟶ [recv b(⦃| ag(a) ‖  m |⦄pk(b))]𝔹 b, (𝕏 a, m)
+| R₂ { Γ } { a b : Agent } { m₁ m₂ : Message σ } { γ : State σ } : NSProof Γ $ ⟨ ι γ ⟩ ⟶ [recv b(⦃| ag(a) ‖  m₁ |⦄pk(b)); recv a(⦃| m₁ ‖  m₂ |⦄pk(a))]𝔹 a, (𝕏 b, (m₁ ‖ m₂))
+| R₃ { Γ } { a b : Agent } { m₁ m₂ : Message σ } { γ : State σ } : NSProof Γ $ ⟨ ι γ ⟩ ⟶ [recv a(⦃| m₁ ‖  m₂ |⦄pk(a)); recv b(⦃| m₂ |⦄pk(b))]𝔹 b, (𝕏 a, m₂)
+
+| MP { Γ } { p q : Formula σ } (hpq : NSProof Γ $ p ⟶ q) (hp : NSProof Γ p) : NSProof Γ q
+| NECα { Γ } { φ : Formula σ } { α : Action σ } (hφ : NSProof Γ φ) : NSProof Γ $ [α]φ
+| NEC𝔹 { Γ } { φ : Formula σ } { a : Agent } (hφ : NSProof Γ φ) : NSProof Γ $ 𝔹 a, φ
+
+notation Γ " ⊢ₙₛ " φ => NSProof Γ φ
 
 @[simp]
-theorem edl_th_1 {σ : Nat} { p q : Formula σ } { α β : Action σ } {a : Agent} { Γ : Context σ } : 
-  (Γ ⊢ₒₛₛ (p ⟶ ([α][β] (𝔹 a, q)))) → 
-  (Γ ⊢ₒₛₛ (p ⟶ ([α][β] (𝕂 a, q)))) := by 
-  intros h
-  admit 
+theorem pl_transitivity_ns {σ : Nat} {p q r : Formula σ} { Γ : Context σ } :
+  (Γ ⊢ₙₛ (p ⟶ q)) →
+  (Γ ⊢ₙₛ (q ⟶ r)) →
+  (Γ ⊢ₙₛ (p ⟶ r)) := by
+  intros hpq hqr
+  have h₁ : Γ ⊢ₙₛ (p ⟶ q ⟶ r) :=
+    NSProof.MP
+      (NSProof.base (ProtocolProof.base Proof.pl₁))
+      hqr
+  have h₂ : Γ ⊢ₙₛ ((p ⟶ q ⟶ r) ⟶ (p ⟶ q) ⟶ (p ⟶ r)) :=
+    NSProof.base (ProtocolProof.base Proof.pl₂)
+  have h₃ : Γ ⊢ₙₛ ((p ⟶ q) ⟶ (p ⟶ r)) :=
+    NSProof.MP h₂ h₁
+  exact NSProof.MP h₃ hpq
 
+@[simp]
+theorem pl2_aux_ns {σ : Nat} {p q r : Formula σ} { Γ : Context σ } :
+  (Γ ⊢ₙₛ (p ⟶ q)) →
+  (Γ ⊢ₙₛ (p ⟶ q ⟶ r)) →
+  (Γ ⊢ₙₛ (p ⟶ r)) := by
+  intros hpq hpqr
+  exact NSProof.MP (NSProof.MP (NSProof.base (ProtocolProof.base Proof.pl₂)) hpqr) hpq
 
-theorem oss { σ : Nat } { Γ : Context σ } { i r e : Agent } { nᵢ : Message σ } : 
-  Γ ⊢ₒₛₛ ((⟨ ι ((i ▷ nᵢ) ⊔ (@γᵢₙᵢₜ σ i r)) ⟩) 
-    ⟶ ([(send i, r(⦃| ag(i) ‖ nᵢ |⦄pk(r))) ; (recv r(⦃| ag(i) ‖ nᵢ |⦄pk(r)))](𝕂 r, ⟨ 𝕏 i, nᵢ ⟩))) :=  by 
-  have S₁ : Γ ⊢ₒₛₛ ⟨ ι ((i ▷ nᵢ) ⊔ (@γᵢₙᵢₜ σ i r)) ⟩ ⟶ [send i,r(⦃| ag(i) ‖  nᵢ |⦄pk(r))]𝔹 i, ⟨ 𝕏 r, nᵢ ⟩ 
-    := OSSProof.S₁ 
-  have H₁ : Γ ⊢ₒₛₛ ⟨ ι ((i ▷ nᵢ) ⊔ (@γᵢₙᵢₜ σ i r)) ⟩ ⟶ [send i,r(⦃| ag(i) ‖  nᵢ |⦄pk(r))]⟨ ι ((e ▷ nᵢ) ⊔ ((i ▷ nᵢ) ⊔ (@γᵢₙᵢₜ σ i r))) ⟩ 
-    := OSSProof.base $ ProtocolProof.H₁ 
-  have hl₀ :  Γ ⊢ₒₛₛ ⟨ ι ((i ▷ nᵢ) ⊔ (@γᵢₙᵢₜ σ i r)) ⟩ ⟶ [send i,r(⦃| ag(i) ‖  nᵢ |⦄pk(r))]((𝔹 i, ⟨ 𝕏 r, nᵢ ⟩) ⋀ (⟨ ι ((e ▷ nᵢ) ⊔ ((i ▷ nᵢ) ⊔ (@γᵢₙᵢₜ σ i r))) ⟩ ))
-    := dl_th_1 S₁ H₁ 
-  have γ₁ : State σ := ((i ▷ nᵢ) ⊔ (@γᵢₙᵢₜ σ i r))
-  have H₂ : Γ ⊢ₒₛₛ ⟨ ι ((e ▷ nᵢ) ⊔ ((i ▷ nᵢ) ⊔ (@γᵢₙᵢₜ σ i r))) ⟩ ⟶ [recv r(⦃| ag(i) ‖ nᵢ |⦄pk(r))]⟨ ι ((r ▷ nᵢ) ⊔ ((e ▷ nᵢ) ⊔ ((i ▷ nᵢ) ⊔ (@γᵢₙᵢₜ σ i r)))) ⟩ 
-    := OSSProof.base $ ProtocolProof.H₂ 
-  have S₂ : Γ ⊢ₒₛₛ ⟨ ι ((e ▷ nᵢ) ⊔ ((i ▷ nᵢ) ⊔ (@γᵢₙᵢₜ σ i r))) ⟩ ⟶ [recv r(⦃| ag(i) ‖ nᵢ |⦄pk(r))](𝔹 r, ⟨ 𝕏 i, nᵢ ⟩) 
-    := OSSProof.S₂ 
-  have hl₁ : Γ ⊢ₒₛₛ ⟨ ι ((e ▷ nᵢ) ⊔ ((i ▷ nᵢ) ⊔ (@γᵢₙᵢₜ σ i r))) ⟩ ⟶ [recv r(⦃| ag(i) ‖ nᵢ |⦄pk(r))]((⟨ ι ((r ▷ nᵢ) ⊔ ((e ▷ nᵢ) ⊔ ((i ▷ nᵢ) ⊔ (@γᵢₙᵢₜ σ i r))))⟩) ⋀ (𝔹 r, ⟨ 𝕏 i, nᵢ ⟩))
-    := dl_th_1 H₂ S₂ 
-  have hl₂_K : Γ ⊢ₒₛₛ [send i,r(⦃| ag(i) ‖  nᵢ |⦄pk(r))] (⟨ ι ((e ▷ nᵢ) ⊔ ((i ▷ nᵢ) ⊔ (@γᵢₙᵢₜ σ i r))) ⟩ ⟶ [recv r(⦃| ag(i) ‖ nᵢ |⦄pk(r))]((⟨ ι ((r ▷ nᵢ) ⊔ ((e ▷ nᵢ) ⊔ ((i ▷ nᵢ) ⊔ (@γᵢₙᵢₜ σ i r))))⟩) ⋀ (𝔹 r, ⟨ 𝕏 i, nᵢ ⟩)))
-    := OSSProof.NECα hl₁
-  have hl₃ : Γ ⊢ₒₛₛ ([send i,r(⦃| ag(i) ‖  nᵢ |⦄pk(r))](⟨ ι ((e ▷ nᵢ) ⊔ ((i ▷ nᵢ) ⊔ (@γᵢₙᵢₜ σ i r))) ⟩)) ⟶ ([send i,r(⦃| ag(i) ‖  nᵢ |⦄pk(r))]( [recv r(⦃| ag(i) ‖ nᵢ |⦄pk(r))]((⟨ ι ((r ▷ nᵢ) ⊔ ((e ▷ nᵢ) ⊔ ((i ▷ nᵢ) ⊔ (@γᵢₙᵢₜ σ i r))))⟩) ⋀ (𝔹 r, ⟨ 𝕏 i, nᵢ ⟩)))) 
-    := OSSProof.MP (OSSProof.base (ProtocolProof.base Proof.Kα)) hl₂_K 
-  have hl₄ : Γ ⊢ₒₛₛ  ⟨ ι ((i ▷ nᵢ) ⊔ (@γᵢₙᵢₜ σ i r)) ⟩ ⟶ ([send i,r(⦃| ag(i) ‖  nᵢ |⦄pk(r))]( [recv r(⦃| ag(i) ‖ nᵢ |⦄pk(r))]((⟨ ι ((r ▷ nᵢ) ⊔ ((e ▷ nᵢ) ⊔ ((i ▷ nᵢ) ⊔ (@γᵢₙᵢₜ σ i r))))⟩) ⋀ (𝔹 r, ⟨ 𝕏 i, nᵢ ⟩)))) 
-    := pl_transitivity H₁ hl₃ 
-  have st₃ : Γ ⊢ₒₛₛ (⟨ι ((r ▷ nᵢ) ⊔ ((e ▷ nᵢ) ⊔ ((i ▷ nᵢ) ⊔ (@γᵢₙᵢₜ σ i r))))⟩) ⟶ (⟨𝕏 r, nᵢ⟩) 
-    := OSSProof.base (ProtocolProof.base Proof.St₃') 
-  have hl₅ : Γ ⊢ₒₛₛ  ⟨ ι ((i ▷ nᵢ) ⊔ (@γᵢₙᵢₜ σ i r)) ⟩ ⟶ ([send i,r(⦃| ag(i) ‖  nᵢ |⦄pk(r))]( [recv r(⦃| ag(i) ‖ nᵢ |⦄pk(r))]((𝔹 r, ⟨ 𝕏 i, nᵢ ⟩))))  
-    := dl_th_2 hl₄ 
-  have hl₆ : Γ ⊢ₒₛₛ  ⟨ ι ((i ▷ nᵢ) ⊔ (@γᵢₙᵢₜ σ i r)) ⟩ ⟶ ([send i,r(⦃| ag(i) ‖  nᵢ |⦄pk(r))]( [recv r(⦃| ag(i) ‖ nᵢ |⦄pk(r))]((𝕂 r, ⟨ 𝕏 i, nᵢ ⟩))))  
-    := edl_th_1 hl₅ 
-  have hl₇ : Γ ⊢ₒₛₛ  ⟨ ι ((i ▷ nᵢ) ⊔ (@γᵢₙᵢₜ σ i r )) ⟩ ⟶ ([send i,r(⦃| ag(i) ‖  nᵢ |⦄pk(r)) ; recv r(⦃| ag(i) ‖ nᵢ |⦄pk(r))]((𝕂 r, ⟨ 𝕏 i, nᵢ ⟩))) 
-    := dl_th_3 hl₆ 
-  exact hl₇ 
+@[simp]
+theorem dl_th_1_ns {σ : Nat} { p q r : Formula σ } { α : Action σ } { Γ : Context σ } :
+  (Γ ⊢ₙₛ (p ⟶ ([α]q))) →
+  (Γ ⊢ₙₛ (p ⟶ ([α]r))) →
+  (Γ ⊢ₙₛ (p ⟶ ([α](q ⋀ r)))) := by
+  intros hq hr
+  have prop_formula : Γ ⊢ (q ⟶ r ⟶ q ⋀ r) := by
+    admit
+  have nec_formula : Γ ⊢ₙₛ ([α](q ⟶ (r ⟶ q ⋀ r))) ⟶ ([α]q) ⟶ ([α](r ⟶ q ⋀ r)) := NSProof.base $ (ProtocolProof.base Proof.Kα)
+  have h₀ : Γ ⊢ₙₛ ([α](q ⟶ (r ⟶ q ⋀ r))) := NSProof.base (ProtocolProof.base (Proof.NECα prop_formula))
+  have h₁ : Γ ⊢ₙₛ ([α]q) ⟶ ([α](r ⟶ q ⋀ r)) := NSProof.MP nec_formula h₀
+  have h₂ : Γ ⊢ₙₛ (p ⟶ ([α](r ⟶ q ⋀ r))) := pl_transitivity_ns hq h₁
+  have nec_formula : Γ ⊢ₙₛ ([α](r ⟶ q ⋀ r)) ⟶ ([α](r)) ⟶ ([α](q ⋀ r)) := NSProof.base (ProtocolProof.base Proof.Kα)
+  have h₃ := pl_transitivity_ns h₂ nec_formula
+  exact pl2_aux_ns hr h₃
+
+theorem ns { σ : Nat } { Γ : Context σ } { i r : Agent } { nᵢ : Message σ } :
+  Γ ⊢ₙₛ ⟨ ι (i ▷ nᵢ ⊔ @γᵢₙᵢₜ σ i r) ⟩
+    ⟶ [recv r(⦃| ag(i) ‖ nᵢ |⦄pk(r))](𝕂 r, (𝕏 i, nᵢ)) := by
+  have H₁ : Γ ⊢ₙₛ ⟨ ι (i ▷ nᵢ ⊔ @γᵢₙᵢₜ σ i r) ⟩ ⟶ [recv r(⦃| ag(i) ‖ nᵢ |⦄pk(r))]𝔹 r, (𝕏 i, nᵢ)
+    := NSProof.R₁'
+  have H₂ : Γ ⊢ₙₛ ⟨ ι (i ▷ nᵢ ⊔ r ▷ nᵢ ⊔ @γᵢₙᵢₜ σ i r) ⟩ ⟶ 𝕏 i, nᵢ
+    := NSProof.base $ ProtocolProof.base $ Proof.St₃
+  let H₃ := @NSProof.NECα _ Γ (⟨ ι (i ▷ nᵢ ⊔ r ▷ nᵢ ⊔ @γᵢₙᵢₜ σ i r) ⟩ ⟶ 𝕏 i, nᵢ) (recv r(⦃| ag(i) ‖ nᵢ |⦄pk(r))) H₂
+  let H₄ := NSProof.base $ ProtocolProof.base $ (@Proof.Kα _ Γ ⟨ ι (i ▷ nᵢ ⊔ r ▷ nᵢ ⊔ @γᵢₙᵢₜ σ i r) ⟩ (𝕏 i, nᵢ) (recv r(⦃| ag(i) ‖ nᵢ |⦄pk(r))))
+  let H₅ := NSProof.MP H₄ H₃
+  have H₆ : Γ ⊢ₙₛ ⟨ ι (i ▷ nᵢ ⊔ @γᵢₙᵢₜ σ i r) ⟩ ⟶ [recv r(⦃| ag(i) ‖ nᵢ |⦄pk(r))]⟨ ι (r ▷ nᵢ ⊔ i ▷ nᵢ ⊔ @γᵢₙᵢₜ σ i r) ⟩
+     := NSProof.base $ ProtocolProof.H₂
+  have H₇ : Γ ⊢ₙₛ ⟨ι (r ▷ nᵢ ⊔ i ▷ nᵢ ⊔ @γᵢₙᵢₜ σ i r)⟩ ⟶ ⟨ι (i ▷ nᵢ ⊔ r ▷ nᵢ ⊔ @γᵢₙᵢₜ σ i r)⟩
+    := NSProof.base $ ProtocolProof.base $ Proof.St₁_left
+  have H₈ := @NSProof.NECα _ Γ (⟨ι (r ▷ nᵢ ⊔ i ▷ nᵢ ⊔ @γᵢₙᵢₜ σ i r)⟩ ⟶ ⟨ι (i ▷ nᵢ ⊔ r ▷ nᵢ ⊔ @γᵢₙᵢₜ σ i r)⟩) (recv r(⦃| ag(i) ‖ nᵢ |⦄pk(r))) H₇
+  have H₉ := NSProof.base $ ProtocolProof.base $ (@Proof.Kα _ Γ ⟨ι (r ▷ nᵢ ⊔ i ▷ nᵢ ⊔ @γᵢₙᵢₜ σ i r)⟩ ⟨ι (i ▷ nᵢ ⊔ r ▷ nᵢ ⊔ @γᵢₙᵢₜ σ i r)⟩ (recv r(⦃| ag(i) ‖ nᵢ |⦄pk(r))))
+  have H₁₀ := NSProof.MP H₉ H₈
+  let H₁₁ := pl_transitivity_ns (pl_transitivity_ns H₆ H₁₀) H₅
+  exact (dl_th_1_ns H₁ H₁₁)
 
 /-
   **AUTOMATED GENERATED MODEL**
@@ -235,7 +448,7 @@ theorem oss { σ : Nat } { Γ : Context σ } { i r e : Agent } { nᵢ : Message 
   **Generate model**
 -/
 
-namespace hidden 
+namespace hidden
 def State (σ : Nat) := List (List $ Message σ)
 
 def EmptyMessage (σ : Nat) : Message σ := Message.empty
@@ -263,256 +476,256 @@ def List.getAtIndex! {α : Type} (list : List α) (i : Nat) (default : α) : α 
 def MessageContext (σ : Nat) := List $ Message σ
 
 def DeductionClosureStep {σ : Nat} (Γ : MessageContext σ) (Γc : MessageContext σ) : MessageContext σ :=
-  match Γ with 
-  | [] => [] 
-  | (m :: tail) => match m with 
+  match Γ with
+  | [] => []
+  | (m :: tail) => match m with
     | ⦃|m'|⦄k => if Γc.contains k && !Γc.contains m' then m' :: m :: DeductionClosureStep tail Γc else m :: DeductionClosureStep tail Γc
-    | m₁ ‖ m₂ => 
-    if Γc.contains (m₁ ‖ m₂) then 
-      if Γc.contains m₁ then 
-        if Γc.contains m₂ then 
-          m :: DeductionClosureStep tail Γc 
-        else 
-          m :: m₂ :: DeductionClosureStep tail Γc 
-      else 
-        if Γc.contains m₂ then 
-          m :: m₁ :: DeductionClosureStep tail Γc 
-        else 
-          m :: m₁ :: m₂ :: DeductionClosureStep tail Γc 
-    else m :: DeductionClosureStep tail Γc 
+    | m₁ ‖ m₂ =>
+    if Γc.contains (m₁ ‖ m₂) then
+      if Γc.contains m₁ then
+        if Γc.contains m₂ then
+          m :: DeductionClosureStep tail Γc
+        else
+          m :: m₂ :: DeductionClosureStep tail Γc
+      else
+        if Γc.contains m₂ then
+          m :: m₁ :: DeductionClosureStep tail Γc
+        else
+          m :: m₁ :: m₂ :: DeductionClosureStep tail Γc
+    else m :: DeductionClosureStep tail Γc
     | _ => m :: DeductionClosureStep tail Γc
 
 set_option maxHeartbeats 800000
 
-def DeductionClosure {σ : Nat} (Γ : MessageContext σ) : MessageContext σ := 
+def DeductionClosure {σ : Nat} (Γ : MessageContext σ) : MessageContext σ :=
   let Γ₀ := DeductionClosureStep Γ Γ
-  let Γ₁ := DeductionClosureStep Γ₀ Γ₀ 
-  let Γ₂ := DeductionClosureStep Γ₁ Γ₁ 
-  Γ₂ 
+  let Γ₁ := DeductionClosureStep Γ₀ Γ₀
+  let Γ₂ := DeductionClosureStep Γ₁ Γ₁
+  Γ₂
 
 
-def MessageInfer {σ : Nat} (Γ : MessageContext σ) (m : Message σ) : Bool := 
+def MessageInfer {σ : Nat} (Γ : MessageContext σ) (m : Message σ) : Bool :=
   let Γ' := DeductionClosure Γ
-  match m with 
+  match m with
   | Message.empty => True
-  | m₁ ‖ m₂ => Γ'.contains (m₁ ‖ m₂) || (Γ'.contains m₁ && Γ'.contains m₂) 
+  | m₁ ‖ m₂ => Γ'.contains (m₁ ‖ m₂) || (Γ'.contains m₁ && Γ'.contains m₂)
   | ⦃|m₁|⦄m₂ => Γ'.contains (⦃|m₁|⦄m₂) || (Γ'.contains m₁ && Γ'.contains m₂)
   | sk(i) => Γ'.contains $ sk(i)
   | pk(i) => Γ'.contains $ pk(i)
   | ag(i) => Γ'.contains $ ag(i)
   | text(t) => Γ'.contains $ text(t)
-  | Message.symmetricKey i j k => Γ'.contains $ Message.symmetricKey i j k 
+  | Message.symmetricKey i j k => Γ'.contains $ Message.symmetricKey i j k
 
-notation Γ " ⊢μ " m => MessageInfer Γ m 
+notation Γ " ⊢μ " m => MessageInfer Γ m
 
-def AwarenessSatisfies {σ : Nat} (M : AutomaticallyGeneratedModel σ) (wIndex : Nat) (agent : Agent) (m : Message σ) : Bool := 
+def AwarenessSatisfies {σ : Nat} (M : AutomaticallyGeneratedModel σ) (wIndex : Nat) (agent : Agent) (m : Message σ) : Bool :=
   let modelAgents : List Agent := M.Agents
   let numberOfAgents : Nat := modelAgents.length
   let zippedAgentList := List.zip modelAgents $ List.range numberOfAgents
   let agentStatePosition : Nat := List.getAtIndex! (List.map (fun (_, pos) => pos) (List.filter  (fun (ag, _) => ag == agent) zippedAgentList) ) 0 0
-  let currentState : State σ := List.getAtIndex! M.States wIndex EmptyState 
+  let currentState : State σ := List.getAtIndex! M.States wIndex EmptyState
   let currentAgentState := List.getAtIndex! currentState agentStatePosition []
-  currentAgentState ⊢μ m 
+  currentAgentState ⊢μ m
 
 def ModalKBStates {σ : Nat} (_ : AutomaticallyGeneratedModel σ) (wIndex : Nat) (agent : Agent) (relation : List $ (Agent × List Nat)) : List Nat :=
   let agentRelation : List $ List Nat := ((relation.filter (fun (ag, _) => ag == agent)).map (fun (_, y) => y)).filter (fun list => List.getAtIndex! list 0 0 == wIndex)
   let accessibleStates : List Nat := agentRelation.map (fun list => List.getAtIndex! list 1 0)
-  accessibleStates 
+  accessibleStates
 
 
-def PDLSendStates {σ : Nat} (_ : AutomaticallyGeneratedModel σ) (wIndex : Nat) (i : Agent) (j : Agent) (m : Message σ) (relation : List $ (Agent × Agent × Message σ × List Nat)) : List Nat := 
+def PDLSendStates {σ : Nat} (_ : AutomaticallyGeneratedModel σ) (wIndex : Nat) (i : Agent) (j : Agent) (m : Message σ) (relation : List $ (Agent × Agent × Message σ × List Nat)) : List Nat :=
   let agentRelation : List $ List Nat := ((relation.filter (fun (agi, agj, msg, _) => agi == i && agj == j && msg == m)).map (fun (_, _, _, y) => y)).filter (fun list => List.getAtIndex! list 0 0 == wIndex)
   let accessibleStates : List Nat := agentRelation.map (fun list => List.getAtIndex! list 1 0)
-  accessibleStates 
+  accessibleStates
 
 def PDLRecvStates {σ : Nat} (_ : AutomaticallyGeneratedModel σ) (wIndex : Nat) (j : Agent) (m : Message σ) (relation : List $ (Agent × Message σ × List Nat)) : List Nat :=
   let agentRelation : List $ List Nat := ((relation.filter (fun (agj, msg, _) => agj == j && msg == m)).map (fun (_, _, y) => y)).filter (fun list => List.getAtIndex! list 0 0 == wIndex)
   let accessibleStates : List Nat := agentRelation.map (fun list => List.getAtIndex! list 1 0)
-  accessibleStates 
+  accessibleStates
 
 def PDLGenStates {σ : Nat} (_ : AutomaticallyGeneratedModel σ) (wIndex : Nat) (j : Agent) (m : Message σ) (relation : List $ (Agent × Message σ × List Nat)) : List Nat :=
   let agentRelation : List $ List Nat := ((relation.filter (fun (agj, msg, _) => agj == j && msg == m)).map (fun (_, _, y) => y)).filter (fun list => List.getAtIndex! list 0 0 == wIndex)
   let accessibleStates : List Nat := agentRelation.map (fun list => List.getAtIndex! list 1 0)
-  accessibleStates 
+  accessibleStates
 
 def SatisfiesAtState {σ : Nat} (M : AutomaticallyGeneratedModel σ) (φ : Formula σ) (wIndex : Nat) : Bool :=
   match φ with
-  | Formula.atom _ => True 
-  | Formula.true => True 
+  | Formula.atom _ => True
+  | Formula.true => True
   | φ ⟶ ψ => (SatisfiesAtState M φ wIndex) → (SatisfiesAtState M ψ wIndex)
-  | ~φ => !(SatisfiesAtState M φ wIndex) 
-  | 𝕏 agent, m => AwarenessSatisfies M wIndex agent m  
-  | 𝔹 agent, φ => 
+  | ~φ => !(SatisfiesAtState M φ wIndex)
+  | 𝕏 agent, m => AwarenessSatisfies M wIndex agent m
+  | 𝔹 agent, φ =>
     let accessibleStates := ModalKBStates M wIndex agent M.R𝔹
     let applySatisfaction := accessibleStates.map (fun accessibleState => SatisfiesAtState M φ accessibleState)
-    applySatisfaction.foldr (fun x y => x && y) True 
-  | [send i, j(m)] φ => 
+    applySatisfaction.foldr (fun x y => x && y) True
+  | [send i, j(m)] φ =>
     let accessibleStates := PDLSendStates M wIndex i j m M.RPDLSend
     let applySatisfaction := accessibleStates.map (fun accessibleState => SatisfiesAtState M φ accessibleState)
-    applySatisfaction.foldr (fun x y => x && y) True 
-  | [recv j(m)] φ => 
-    let accessibleStates := PDLRecvStates M wIndex j m M.RPDLRecv 
+    applySatisfaction.foldr (fun x y => x && y) True
+  | [recv j(m)] φ =>
+    let accessibleStates := PDLRecvStates M wIndex j m M.RPDLRecv
     let applySatisfaction := accessibleStates.map (fun accessibleState => SatisfiesAtState M φ accessibleState)
-    applySatisfaction.foldr (fun x y => x && y) True 
-  | _ => True 
+    applySatisfaction.foldr (fun x y => x && y) True
+  | _ => True
 
 notation M " at " w " ⊧ " φ => SatisfiesAtState M φ w
 
-def Satisfies {σ : Nat} (M : AutomaticallyGeneratedModel σ) (φ : Formula σ) : Bool := 
-  let allStates := List.range $ M.States.length 
+def Satisfies {σ : Nat} (M : AutomaticallyGeneratedModel σ) (φ : Formula σ) : Bool :=
+  let allStates := List.range $ M.States.length
   let satisfiesAllStates := allStates.map (fun state => M at state ⊧ φ)
-  satisfiesAllStates.foldr (fun x y => x && y) True 
+  satisfiesAllStates.foldr (fun x y => x && y) True
 
-notation M " ⊧ " φ => Satisfies M φ 
+notation M " ⊧ " φ => Satisfies M φ
 
 
-structure ProtocolAction (σ : Nat) where 
+structure ProtocolAction (σ : Nat) where
   Sender: Agent
   Receiver: Agent
-  Message: Message σ 
+  Message: Message σ
 
-instance EmptyProtocolAction {σ : Nat} : ProtocolAction σ := 
+instance EmptyProtocolAction {σ : Nat} : ProtocolAction σ :=
 {
   Sender := "",
   Receiver := "",
-  Message := Message.empty 
-}  
+  Message := Message.empty
+}
 
 structure Protocol (σ : Nat) where
-  Agents : List Agent 
+  Agents : List Agent
   SymmetricKeys : List $ (Agent × Agent × Message σ)
-  Specification : List $ ProtocolAction σ 
+  Specification : List $ ProtocolAction σ
 
-def GetAllSubMessages {σ : Nat} (m : Message σ) : List $ Message σ := 
-  match m with 
-  | Message.empty => [] 
+def GetAllSubMessages {σ : Nat} (m : Message σ) : List $ Message σ :=
+  match m with
+  | Message.empty => []
   | text(t) => [text(t) ]
   | ag(i) => [ag(i) ]
   | Message.symmetricKey k i j => [Message.symmetricKey k i j]
   | pk(i) => [pk(i) ]
   | sk(i) => [sk(i) ]
-  | ⦃|m|⦄k => GetAllSubMessages m ++ [k] 
-  | m₁ ‖ m₂ => GetAllSubMessages m₁ ++ GetAllSubMessages m₂   
+  | ⦃|m|⦄k => GetAllSubMessages m ++ [k]
+  | m₁ ‖ m₂ => GetAllSubMessages m₁ ++ GetAllSubMessages m₂
 
-def GetAllMessagesFromList {σ : Nat} (list : List $ Message σ) : List $ Message σ := 
-  match list with 
-  | [] => [] 
-  | (message :: tail) => 
-    match message with 
-    | Message.empty => tail 
-    | text(t) => text(t) :: tail 
-    | ag(i) => ag(i) :: tail 
-    | Message.symmetricKey k i j => (Message.symmetricKey k i j) :: tail 
-    | pk(i) => pk(i) :: tail 
-    | sk(i) => sk(i) :: tail 
-    | ⦃|m|⦄k => GetAllSubMessages (⦃|m|⦄k) ++ [⦃|m|⦄k] ++ tail 
-    | m₁ ‖ m₂ => GetAllSubMessages (m₁ ‖ m₂) ++ [m₁ ‖ m₂] ++ tail 
-
-def List.removeDuplicates {α : Type} [BEq α] (list : List α) : List α := 
-  match list with 
+def GetAllMessagesFromList {σ : Nat} (list : List $ Message σ) : List $ Message σ :=
+  match list with
   | [] => []
-  | (head :: tail) => if tail.contains head then tail else head :: tail 
+  | (message :: tail) =>
+    match message with
+    | Message.empty => tail
+    | text(t) => text(t) :: tail
+    | ag(i) => ag(i) :: tail
+    | Message.symmetricKey k i j => (Message.symmetricKey k i j) :: tail
+    | pk(i) => pk(i) :: tail
+    | sk(i) => sk(i) :: tail
+    | ⦃|m|⦄k => GetAllSubMessages (⦃|m|⦄k) ++ [⦃|m|⦄k] ++ tail
+    | m₁ ‖ m₂ => GetAllSubMessages (m₁ ‖ m₂) ++ [m₁ ‖ m₂] ++ tail
+
+def List.removeDuplicates {α : Type} [BEq α] (list : List α) : List α :=
+  match list with
+  | [] => []
+  | (head :: tail) => if tail.contains head then tail else head :: tail
 
 
-def AppendAgentNewKnowledge {σ : Nat} (P : Protocol σ) (agent : Agent) (currentState : State σ) (newKnowledge : List $ Message σ) : State σ := 
-  let agentsNumber := P.Agents.length 
+def AppendAgentNewKnowledge {σ : Nat} (P : Protocol σ) (agent : Agent) (currentState : State σ) (newKnowledge : List $ Message σ) : State σ :=
+  let agentsNumber := P.Agents.length
   let agentsPositions := List.zip P.Agents $ List.range $ agentsNumber
   let agentPosition := List.getAtIndex! (List.map (fun (_, pos) => pos) (List.filter (fun (ag, _) => ag == agent) agentsPositions)) 0 0
-  let stateForAgents := currentState.zip $ List.range $ agentsNumber 
-  let newState := stateForAgents.map (fun (ik, pos) => 
-    if pos == agentPosition then List.removeDuplicates (List.append ik newKnowledge) else ik 
+  let stateForAgents := currentState.zip $ List.range $ agentsNumber
+  let newState := stateForAgents.map (fun (ik, pos) =>
+    if pos == agentPosition then List.removeDuplicates (List.append ik newKnowledge) else ik
   )
   newState
 
-def getAtIndexAux! : List α → Nat → Nat → α → α := fun la currentIndex searchedIndex default => 
-  match la with 
-  | [] => default 
-  | (x::xs) => if currentIndex == searchedIndex then x else getAtIndexAux! xs (currentIndex + 1) searchedIndex default 
+def getAtIndexAux! : List α → Nat → Nat → α → α := fun la currentIndex searchedIndex default =>
+  match la with
+  | [] => default
+  | (x::xs) => if currentIndex == searchedIndex then x else getAtIndexAux! xs (currentIndex + 1) searchedIndex default
 
-def getAtIndex! : List α → Nat → α → α := fun la index default => getAtIndexAux! la 0 index default 
-  
+def getAtIndex! : List α → Nat → α → α := fun la index default => getAtIndexAux! la 0 index default
+
 def BuildFromActions {σ : Nat} (P : Protocol σ) (currentStateIndex : Nat) (states : List $ State σ) (statesLeft : Nat)
-  : (List $ State σ) 
-  × (List $ (Agent × Agent × Message σ × List Nat)) 
-  × (List $ (Agent × Message σ × List Nat)) := 
-  match statesLeft with 
+  : (List $ State σ)
+  × (List $ (Agent × Agent × Message σ × List Nat))
+  × (List $ (Agent × Message σ × List Nat)) :=
+  match statesLeft with
   | 0 => ([], [], [])
-  | n + 1 => 
+  | n + 1 =>
     let currentAction := List.getAtIndex! P.Specification currentStateIndex ({ Sender := "", Receiver := "", Message := Message.empty })
-    let sender := currentAction.Sender 
-    let receiver := currentAction.Receiver 
-    let message := currentAction.Message 
-    let lastState := List.getAtIndex! states (states.length - 1) EmptyState 
-    let newState := AppendAgentNewKnowledge P sender lastState [message] 
-  
-    let newUpdatedState := 
-      if currentStateIndex != 0 then 
-        let lastAction := List.getAtIndex! P.Specification (currentStateIndex - 1) ({ Sender := "", Receiver := "", Message := Message.empty })
-        let lastReceiver := lastAction.Receiver 
-        let lastMessage := lastAction.Message 
-        AppendAgentNewKnowledge P lastReceiver newState [lastMessage]
-      else newState 
+    let sender := currentAction.Sender
+    let receiver := currentAction.Receiver
+    let message := currentAction.Message
+    let lastState := List.getAtIndex! states (states.length - 1) EmptyState
+    let newState := AppendAgentNewKnowledge P sender lastState [message]
 
-    (newUpdatedState :: (BuildFromActions P (currentStateIndex + 1) (states.append [newUpdatedState]) n).fst, 
-    if message != Message.empty then 
-      ((sender, receiver, message, [currentStateIndex, currentStateIndex + 1]) :: (BuildFromActions P (currentStateIndex + 1) (states.append [newUpdatedState]) n).snd.fst) 
+    let newUpdatedState :=
+      if currentStateIndex != 0 then
+        let lastAction := List.getAtIndex! P.Specification (currentStateIndex - 1) ({ Sender := "", Receiver := "", Message := Message.empty })
+        let lastReceiver := lastAction.Receiver
+        let lastMessage := lastAction.Message
+        AppendAgentNewKnowledge P lastReceiver newState [lastMessage]
+      else newState
+
+    (newUpdatedState :: (BuildFromActions P (currentStateIndex + 1) (states.append [newUpdatedState]) n).fst,
+    if message != Message.empty then
+      ((sender, receiver, message, [currentStateIndex, currentStateIndex + 1]) :: (BuildFromActions P (currentStateIndex + 1) (states.append [newUpdatedState]) n).snd.fst)
     else (BuildFromActions P (currentStateIndex + 1) (states.append [newUpdatedState]) n).snd.fst,
-    if message != Message.empty then 
-      ((receiver, message, [currentStateIndex, currentStateIndex + 1]) :: (BuildFromActions P (currentStateIndex + 1) (states.append [newUpdatedState]) n).snd.snd) 
+    if message != Message.empty then
+      ((receiver, message, [currentStateIndex, currentStateIndex + 1]) :: (BuildFromActions P (currentStateIndex + 1) (states.append [newUpdatedState]) n).snd.snd)
     else (BuildFromActions P (currentStateIndex + 1) (states.append [newUpdatedState]) n).snd.snd
     )
 
-def BuildModel {σ : Nat} (P : Protocol σ) : AutomaticallyGeneratedModel σ := 
-  let specification := P.Specification 
-  let agentsNumber := P.Agents.length 
+def BuildModel {σ : Nat} (P : Protocol σ) : AutomaticallyGeneratedModel σ :=
+  let specification := P.Specification
+  let agentsNumber := P.Agents.length
   let agentsPositions := List.zip P.Agents $ List.range $ agentsNumber
 
   let initialAction := getAtIndex! specification 0 EmptyProtocolAction
-  let agentsInitialKnowledgeEmpty : List $ List $ Message σ := List.replicate agentsNumber [] 
+  let agentsInitialKnowledgeEmpty : List $ List $ Message σ := List.replicate agentsNumber []
   let initialAgentPosition := getAtIndex! ((agentsPositions.filter (fun (ag, _) => ag == initialAction.Sender)).map (fun (_, pos) => pos)) 0 0
 
-  let agentsInitialKnowledge := ((agentsInitialKnowledgeEmpty.zip (List.range agentsNumber)).map (fun (ik, agentPos) => 
+  let agentsInitialKnowledge := ((agentsInitialKnowledgeEmpty.zip (List.range agentsNumber)).map (fun (ik, agentPos) =>
     if agentPos == initialAgentPosition then ik.append [initialAction.Message] else ik.append []))
 
-  let agentsInitialKnowledgeKeys := (agentsInitialKnowledge.zip (List.range agentsNumber)).map (fun (ik, pos) => 
+  let agentsInitialKnowledgeKeys := (agentsInitialKnowledge.zip (List.range agentsNumber)).map (fun (ik, pos) =>
     let agentByPos := getAtIndex! ((agentsPositions.filter (fun ((_ : Agent), y) => y == pos)).map (fun ((x : Agent), (_ : Nat)) => x)) 0 ""
     let searchInSymmetricKeys := P.SymmetricKeys.filter (fun ((x : Agent), (y : Agent), (_ : Message σ)) => x == agentByPos || y == agentByPos)
-    let key := if searchInSymmetricKeys.length > 0 then (getAtIndex! searchInSymmetricKeys 0 (("", "", Message.empty) : Agent × Agent × Message σ)).snd.snd else Message.empty 
+    let key := if searchInSymmetricKeys.length > 0 then (getAtIndex! searchInSymmetricKeys 0 (("", "", Message.empty) : Agent × Agent × Message σ)).snd.snd else Message.empty
     let otherAgentsPublicKeys : List $ Message σ := (P.Agents.filter (fun ag => ag != agentByPos)).map (fun ag => pk(ag))
     if key != Message.empty then (ik.append [key, sk(agentByPos), pk(agentByPos) ]).append otherAgentsPublicKeys else (ik.append [sk(agentByPos), pk(agentByPos) ]).append otherAgentsPublicKeys
     )
-  
+
   let initialState : State σ := agentsInitialKnowledgeKeys
 
   let result := BuildFromActions P 0 [initialState] (specification.length + 1)
 
-  let states := result.fst 
-  let pdlRelationSend := result.snd.fst 
+  let states := result.fst
+  let pdlRelationSend := result.snd.fst
 
-  let firstOccuranceForEveryAgent := P.Agents.map (fun agent => 
-    let firstState : Nat := getAtIndex! (getAtIndex! ((pdlRelationSend.filter (fun (ag, _, _, _) => ag == agent)).map (fun (_, _, _, ls) => ls)) 0 []) 0 0 
+  let firstOccuranceForEveryAgent := P.Agents.map (fun agent =>
+    let firstState : Nat := getAtIndex! (getAtIndex! ((pdlRelationSend.filter (fun (ag, _, _, _) => ag == agent)).map (fun (_, _, _, ls) => ls)) 0 []) 0 0
     (agent, firstState)
   )
 
-  let numberOfStates := states.length 
+  let numberOfStates := states.length
 
-  let knowledge_relation := firstOccuranceForEveryAgent.map (fun (ag, initialAgentState) => 
-    let allStates := List.range numberOfStates 
+  let knowledge_relation := firstOccuranceForEveryAgent.map (fun (ag, initialAgentState) =>
+    let allStates := List.range numberOfStates
     let agentStates := (List.foldr (fun x y => x ++ y) [] $ (allStates.map (fun x => allStates.map (fun y => if x <= y then [x, y] else []))))
-    let agentListFiltered := agentStates.filter (fun (list : List Nat) => getAtIndex! list 0 0 >= initialAgentState) 
+    let agentListFiltered := agentStates.filter (fun (list : List Nat) => getAtIndex! list 0 0 >= initialAgentState)
     (agentListFiltered.map (fun list => (ag, list))).filter (fun (_, list) => list != [])
   )
 
-  let knowledge := List.foldr (fun x y => x ++ y) [] knowledge_relation 
+  let knowledge := List.foldr (fun x y => x ++ y) [] knowledge_relation
 
-  let belief_relation := firstOccuranceForEveryAgent.map (fun (ag, initialAgentState) => 
-    let allStates := List.range numberOfStates 
+  let belief_relation := firstOccuranceForEveryAgent.map (fun (ag, initialAgentState) =>
+    let allStates := List.range numberOfStates
     let agentStates := (List.foldr (fun x y => x ++ y) [] $ (allStates.map (fun x => allStates.map (fun y => if x < y then [x, y] else [])))) ++ ([[getAtIndex! allStates (allStates.length - 1) 0, getAtIndex! allStates (allStates.length - 1) 0]])
-    let agentListFiltered := agentStates.filter (fun (list : List Nat) => getAtIndex! list 0 0 >= initialAgentState) 
+    let agentListFiltered := agentStates.filter (fun (list : List Nat) => getAtIndex! list 0 0 >= initialAgentState)
     (agentListFiltered.map (fun list => (ag, list))).filter (fun (_, list) => list != [])
   )
 
-  let belief := List.foldr (fun x y => x ++ y) [] belief_relation 
+  let belief := List.foldr (fun x y => x ++ y) [] belief_relation
 
   {
     Agents := P.Agents,
@@ -530,7 +743,7 @@ def BuildModel {σ : Nat} (P : Protocol σ) : AutomaticallyGeneratedModel σ :=
 -/
 
 section OSS
-  instance OSS {σ : Nat} : Protocol σ := 
+  instance OSS {σ : Nat} : Protocol σ :=
   {
     Agents := ["i", "r"]
     SymmetricKeys := []
@@ -541,7 +754,18 @@ section OSS
 
   def OSSModel {σ : Nat} : AutomaticallyGeneratedModel σ := BuildModel OSS
 
-  #reduce OSSModel 
+  #reduce OSSModel
+
+  -- { Agents := ["i", "r"],
+  -- States :=
+  --   [[[ sk( "i" ) , pk( "i" ) , pk( "r" ) , ⦃| text( "i" ) ‖ text( "ni" ) |⦄ pk( "r" ) ],
+  --       [ sk( "r" ) , pk( "r" ) , pk( "i" ) ]],
+  --     [[ sk( "i" ) , pk( "i" ) , pk( "r" ) , ⦃| text( "i" ) ‖ text( "ni" ) |⦄ pk( "r" ) , Message.empty],
+  --       [ sk( "r" ) , pk( "r" ) , pk( "i" ) , ⦃| text( "i" ) ‖ text( "ni" ) |⦄ pk( "r" ) ]]],
+  -- R𝕂 := [("i", [0, 0]), ("i", [0, 1]), ("i", [1, 1]), ("r", [0, 0]), ("r", [0, 1]), ("r", [1, 1])],
+  -- R𝔹 := [("i", [0, 1]), ("i", [1, 1]), ("r", [0, 1]), ("r", [1, 1])],
+  -- RPDLSend := [("i", "r", ⦃| text( "i" ) ‖ text( "ni" ) |⦄ pk( "r" ) , [0, 1])],
+  -- RPDLRecv := [("r", ⦃| text( "i" ) ‖ text( "ni" ) |⦄ pk( "r" ) , [0, 1])], RPDLGen := [] }
 
   #reduce OSSModel ⊧ 𝕏 "i", #"ni"#
 
@@ -549,12 +773,12 @@ section OSS
 
   #reduce OSSModel ⊧ [recv "r"(⦃|#"i"# ‖ #"ni"#|⦄pk("r"))] ((𝕂 "i", 𝕏 "r", #"ni"#) ⋀ (𝕂 "r", 𝕏 "i", #"ni"#))
 
-  
+
 
 end OSS
 
 section OSSE
-  instance OSSE {σ : Nat} : Protocol σ := 
+  instance OSSE {σ : Nat} : Protocol σ :=
   {
     Agents := ["i", "r", "e"]
     SymmetricKeys := []
@@ -565,7 +789,7 @@ section OSSE
 
   def OSSEModel {σ : Nat} : AutomaticallyGeneratedModel σ := BuildModel OSSE
 
-  #reduce OSSEModel 
+  #reduce OSSEModel
 
   #reduce OSSEModel ⊧ [recv "r"(⦃|#"i"# ‖ #"ni"#|⦄pk("r"))] ((𝕂 "i", 𝕏 "r", #"ni"#) ⋀ (𝕂 "r", 𝕏 "i", #"ni"#))
 
@@ -576,10 +800,10 @@ end OSSE
 -/
 
 section NeedhamSchroeder
-  instance NeedhamSchroeder {σ : Nat} : Protocol σ := 
+  instance NeedhamSchroeder {σ : Nat} : Protocol σ :=
   {
     Agents := ["i", "r"]
-    SymmetricKeys := [] 
+    SymmetricKeys := []
     Specification := [
       { Sender := "i", Receiver := "r", Message := ⦃|ag("i") ‖ #"ni"#|⦄pk("r") },
       { Sender := "r", Receiver := "r", Message := ⦃|#"ni"# ‖ #"nr"# |⦄pk("i") },
@@ -595,15 +819,15 @@ section NeedhamSchroeder
   -- true
 
   -- #reduce NeedhamSchroederModel ⊧ [recv "r"(⦃|ag("i") ‖ #"ni"#|⦄pk("r"))] ([recv "i"(⦃|#"ni"# ‖ #"nr"# |⦄pk("i"))] 𝕂 "i", 𝕏 "r", #"nr"#)
-  -- true 
+  -- true
 
 end NeedhamSchroeder
 
 section NeedhamSchroederMitM
-  instance NeedhamSchroederMitM {σ : Nat} : Protocol σ := 
+  instance NeedhamSchroederMitM {σ : Nat} : Protocol σ :=
   {
     Agents := ["i", "r", "e"]
-    SymmetricKeys := [] 
+    SymmetricKeys := []
     Specification := [
       { Sender := "i", Receiver := "e", Message := ⦃|ag("i") ‖ #"ni"#|⦄pk("e") },
       { Sender := "e", Receiver := "r", Message := ⦃|ag("i") ‖ #"ni"#|⦄pk("r") },
@@ -619,9 +843,9 @@ section NeedhamSchroederMitM
   #reduce NeedhamSchroederMitMModel
 
   -- #reduce NeedhamSchroederMitMModel ⊧ [recv "r"(⦃|ag("i") ‖ #"ni"#|⦄pk("r"))] 𝕂 "r", 𝕏 "i", #"ni"#
-  -- true 
+  -- true
 
   -- #reduce NeedhamSchroederMitMModel ⊧ 𝕂 "i", 𝕏 "r", #"ni"#
-  -- false 
+  -- false
 end NeedhamSchroederMitM
-end hidden 
+end hidden
